Alg/ListProps/Sorted/Intersect.lean
@@ -249,9 +249,9 @@ theorem List.sorted_intersect.of_contains [Compare α] : ∀(as bs: List α) (x:
     match as_con with
     | .inl h =>
       simp at h
-      have := List.contains_sorted bs_con bs_sort
+      have := List.sorted.contains bs_con bs_sort
       rw [h] at this
-      have := Compare.not_lt_and_le _ _ a_ord_b
+      have := Compare.not_lt_and_le a_ord_b
       contradiction
     | .inr _ => assumption
     assumption
@@ -293,9 +293,9 @@ theorem List.sorted_intersect.of_contains [Compare α] : ∀(as bs: List α) (x:
     match bs_con with
     | .inl h =>
       simp at h
-      have := List.contains_sorted as_con as_sort
+      have := List.sorted.contains as_con as_sort
       rw [h] at this
-      have := Compare.not_lt_and_le _ _ (Compare.flip a_ord_b)
+      have := Compare.not_lt_and_le (Compare.flip a_ord_b)
       contradiction
     | .inr _ => assumption
     assumption
