Alg/Nat/PrimeFactors/Intersect.lean
@@ -44,7 +44,7 @@ theorem list_product.of_sorted_intersect :
       assumption
     }
     {
-      have not_con := List.not_contains_sorted a_ord_b bs_sort
+      have not_con := List.sorted.not_contains a_ord_b bs_sort
       generalize b_fact_def:PrimeFactorization.mk (b::bs) bs_primes rfl bs_sort = b_fact
       have b_complete := b_fact.is_complete a as_primes.left
       rw [←b_fact_def] at b_complete
@@ -87,7 +87,7 @@ theorem list_product.of_sorted_intersect :
       exact bs_primes.right
     }
     {
-      have not_con := List.not_contains_sorted (Compare.flip a_ord_b) as_sort
+      have not_con := List.sorted.not_contains (Compare.flip a_ord_b) as_sort
       generalize a_fact_def:PrimeFactorization.mk (a::as) as_primes rfl as_sort = a_fact
       have a_complete := a_fact.is_complete b bs_primes.left
       rw [←a_fact_def] at a_complete
